viz/gaussian_walk.py
@@ -1,0 +1,15 @@
+def gaussian_walk(length):
+    z = 0j
+    points = []
+
+    for n in range(length):
+        s2 = n.bit_count()
+        u = 1j ** s2
+        c = 1j * (1 - u) / (1 - 1j)
+        W = 2 * z + c
+        H = 4 * n + s2 % 4
+        P = round(W.real), round(W.imag), H
+        points.append(P)
+        z += u
+
+    return points
